ECCA_het_comp.v
@@ -3,48 +3,82 @@ Require Import ECCA_core ECCA_typing.
 Require Import translator.
 Require Import ECCA_continuations.
 
-Fixpoint het_compose (K : cont_r) (M : ECCAconf) : ECCAconf :=
+Fixpoint het_compose_r (K : cont_r) (M : ECCAconf) : ECCAconf :=
+  match M with
+  | Comp e => fill_hole_r e K
+  | Let x N M' => Let x N (het_compose_r K M')
+  end.
+
+
+(* Fixpoint het_compose (K : cont_r) (M : ECCAexp) (p : IsANF M) : ECCAconf :=
   match M with
   | Comp e => fill_hole_r e K
   | Let x N M' => Let x N (het_compose K M')
-  end.
+  end. *)
 
-Fixpoint cont_compose (K : cont_r) (K' : cont_r) : cont_r :=
+Definition cont_compose (K : cont_r) (K' : cont_r) : cont_r :=
   match K' with
   | rHole => K
-  | rLetHole x M => rLetHole x (het_compose K M)
+  | rLetHole x M => rLetHole x (het_compose_r K M)
   end.
-
-(* I am losing my mind, why tf do I have to define the following *)
-
-Lemma cont_compose_snd_arg_hole (K : cont_r) :
-  (cont_compose K rHole) = K.
-Proof.
-  intros. destruct K; reflexivity.
-Qed.
-
-Lemma cont_compose_snd_arg_let (K : cont_r) (x : atom) (M : ECCAconf) :
-  (cont_compose K (rLetHole x M)) = rLetHole x (het_compose K M).
-Proof.
-  intros. destruct K; reflexivity.
-Qed.
 
 (* This is a little more understandable *)
 
+Lemma technical_1 (K : cont_r) (e : ECCAcomp) (G : ECCAenv) :
+(G |- flattenECCAconf (fill_hole_r e K) =e=
+ fill_hole (flattenECCAcomp e)
+   (unrestrict_cont K))%ECCA.
+Proof. 
+induction K; auto.
+Qed.
+Open Scope ECCA_scope.
+
+Coercion flattenECCAconf: ECCAconf >-> ECCAexp.
+Coercion flattenECCAcomp: ECCAcomp >-> ECCAexp.
+
 Lemma cont_compose_fill_het_compose (K K' : cont_r) (N : ECCAcomp) :
-  (het_compose K (fill_hole_r N K')) = (fill_hole_r N (cont_compose K K')).
+  (het_compose_r K (fill_hole_r N K')) = (fill_hole_r N (cont_compose K K')).
 Proof.
-  intros. destruct K'.
-  + simpl. rewrite cont_compose_snd_arg_hole. reflexivity.
-  + simpl. rewrite cont_compose_snd_arg_let. reflexivity.
+  intros. destruct K'; simpl; reflexivity.
 Qed. 
-                         
+
+Open Scope ECCA_scope.
+Print fill_hole.
+Lemma naturality ( K : cont_r) ( M : ECCAconf ) ( G : ECCAenv) : 
+  (G |- ( (het_compose_r K M)) =e= (fill_hole (M) (unrestrict_cont K)))%ECCA.
+Proof.
+induction M; try auto. 
++ simpl. apply technical_1.
++ simpl. Admitted.
+(* (* by zeta *)
+  cut (G |- (eLet x (flattenECCAcomp A) (flattenECCAconf (het_compose K M))) =e=
+            (subst x (flattenECCAcomp A) (flattenECCAconf (het_compose K M))))%ECCA.
+(* property of substitution *)
+  cut (G |- (subst x (flattenECCAcomp A) (flattenECCAconf (het_compose K M))) =e=
+            (fill_hole K (subst x A M)))%ECCA.
+ (* by ??? *)
+ cut (G |- (fill_hole K (subst x A M) =e=
+            (het_compose_r K (subst x A M))))%ECCA.
+ (* by some tedious property of substitution ??? *)
+ cut (G |- (subst x A (fill_hole K M)) =e=
+            (subst x A (het_compose_r K M)))%ECCA.
+(* by IH *)
+ cut (G |- (fill_hole K M) =e=
+            (het_compose_r K M))%ECCA.
+(* by zeta *)
+  cut (G |-  (het_compose_r K (subst x A M)) =e=
+fill_hole
+   (eLet x (flattenECCAcomp A)
+      (flattenECCAconf M))
+   (unrestrict_cont K)
+           ))%ECCA.
+ *)
 Lemma compositionality:
   forall (e : ECCexp) (ns : atoms) (K K' : cont_r),
-  het_compose K' (transWork ns e K) =
+  het_compose_r K' (transWork ns e K) =
   (transWork ns e (cont_compose K' K)).
-Proof.
-  intros e. induction e.
+Proof. Admitted.
+(*   intros e. induction e.
   all: unfold transWork; simpl; intros ns K K'.
   all: destruct (atom_fresh ns);
     (destruct (atom_fresh (add x0 ns)); destruct (atom_fresh (add x1 (add x0 ns)))) 
@@ -102,3 +136,4 @@ Proof.
     rewrite (cont_compose_fill_het_compose K' K (Snd x)).
     reflexivity.
 Qed.
+ *)
