ECCA_subst.v
@@ -116,4 +116,4 @@ Qed.
 Definition subst (x: atom) (arg body: ECCAexp):= substWork x arg body.
 Search "substWork_eq".
 
-Notation "b '[' a '/' x ']'":= (subst x a b) (at level 50): ECCA_scope. 
+Notation "b '[' a '/' x ']'":= (subst x a b) (at level 50, a at level 50): ECCA_scope. 
