ECCA_trans_preservation.v
@@ -2,19 +2,36 @@ Require Import ECC.
 Require Import ECCA_core ECCA_typing ECCA_equiv ECCA_continuations.
 Require Import translator.
 Require Import ECCA_het_comp.
+Require Import ECCA_key_lemmas.
 
-Locate ECCAcont.
-
-(* Lemma 1.1 *)
-Lemma strong_trans_preservation 
-(g: ECCenv) (e A: ECCexp) 
+Definition P1 (g : ECCenv) (e A : ECCexp) (h : ECC_has_type g e A) := (
+(forall
 (g': ECCAenv) (K: cont_r) 
-(B N: ECCAexp):
-
-(ECC_Env_WF g -> ECCA_Env_WF (transEnv g))
-/\
-(ECC_has_type g e A ->
+(B N: ECCAexp),
 ECCA_cont_has_type (appendEnv (transEnv g) g') (unrestrict_cont K) (Cont N (flattenECCAconf (trans A)) B) ->
 ECCA_Equiv (appendEnv (transEnv g) g') (flattenECCAconf (trans e)) N ->
-ECCA_has_type (appendEnv (transEnv g) g') (flattenECCAconf (het_compose K (trans e) )) B). 
+ECCA_has_type (appendEnv (transEnv g) g') (flattenECCAconf (transWork (ECC.FV e) e K)) B)).
+
+Definition P2 (g : ECCenv) (h : ECC_Env_WF g) := ECCA_Env_WF (transEnv g).
+
+Combined Scheme ECC_type_env_comb from ECC_env_type_mut, ECC_type_env_mut.
+
+Lemma strong_trans_preservation :
+
+(forall (g : ECCenv) (h : ECC_Env_WF g),  ECCA_Env_WF (transEnv g)) /\
+(forall (g : ECCenv) (e A : ECCexp) (H : ECC_has_type g e A), 
+forall (g': ECCAenv) (K: cont_r) 
+(B N: ECCAexp),
+ECCA_cont_has_type (appendEnv (transEnv g) g') (unrestrict_cont K) (Cont N (flattenECCAconf (trans A)) B) ->
+ECCA_Equiv (appendEnv (transEnv g) g') (flattenECCAconf (trans e)) N ->
+ECCA_has_type (appendEnv (transEnv g) g') (flattenECCAconf (transWork (ECC.FV e) e K)) B).
 Proof.
+intros.
+simple apply ECC_type_env_comb; intros.
+- unfold transWork. simpl.  destruct (atom_fresh empty). destruct (atom_fresh (add x empty)). destruct (atom_fresh (add x0 (add x empty))).
+  cut (ECCA_has_type (transEnv g) (Uni uProp) (Uni (uType 0))).
+  + shelve. eapply Cut. ...
+  + auto.
+-
+-
+Qed.
